src/SI/ISQ_Algebra.thy
@@ -25,7 +25,7 @@ lemma scaleQ_inv: "-a \<odot> x = a \<odot> -x"
   by si_calc
 
 lemma scaleQ_as_qprod: "a \<odot> x \<cong>\<^sub>Q (a \<odot> \<one>) \<^bold>\<cdot> x"
-  by si_calc
+  by (si_simp)
 
 lemma mult_scaleQ_left [simp]: "(a \<odot> x) \<^bold>\<cdot> y = a \<odot> x \<^bold>\<cdot> y"
   by (si_simp add: mult.assoc)
@@ -53,7 +53,7 @@ text\<open>The following weak congruences will allow for replacing equivalences 
 lemma qtimes_weak_cong_left:
   assumes "x \<cong>\<^sub>Q y"
   shows  "x\<^bold>\<cdot>z \<cong>\<^sub>Q y\<^bold>\<cdot>z"
-  using assms by si_calc
+  using assms by si_simp
 
 lemma qtimes_weak_cong_right:
   assumes "x \<cong>\<^sub>Q y"
@@ -65,11 +65,16 @@ lemma qinverse_weak_cong:
   shows   "x\<^sup>-\<^sup>\<one> \<cong>\<^sub>Q y\<^sup>-\<^sup>\<one>"
   using assms by si_calc
 
+lemma scaleQ_cong:
+  assumes "y \<cong>\<^sub>Q z"
+  shows "x \<odot> y \<cong>\<^sub>Q x \<odot> z"
+  using assms by si_calc
+
 lemma qinverse_qinverse: "x\<^sup>-\<^sup>\<one>\<^sup>-\<^sup>\<one> \<cong>\<^sub>Q x"
   by si_calc
 
 lemma qinverse_nonzero_iff_nonzero: "x\<^sup>-\<^sup>\<one> = 0 \<longleftrightarrow> x = 0"
-  by si_calc
+  by (auto, si_calc+)
 
 lemma qinverse_qtimes: "(x \<^bold>\<cdot> y)\<^sup>-\<^sup>\<one> \<cong>\<^sub>Q x\<^sup>-\<^sup>\<one> \<^bold>\<cdot> y\<^sup>-\<^sup>\<one>"
   by si_calc
